timeprot-subset-invs: Resurrect obj-based defs + add @lsf37's new TA one
Signed-off-by: Robert Sison <robert.sison@unimelb.edu.au>

proof/infoflow/timeprotection/CachePartitionIntegrity.thy
@@ -8,6 +8,8 @@ theory CachePartitionIntegrity
 imports InfoFlow.ADT_IF
 begin
 
+section \<open> Kernel heap-agnostic subset property definitions \<close>
+
 context Arch begin
 
 definition policy_owned_addrs :: "'a PAS \<Rightarrow> domain \<Rightarrow> obj_ref set" where
@@ -104,8 +106,6 @@ lemma owned_to_accessible_addrs_well_partitioned:
   apply(force simp:owned_addrs_well_partitioned_def policy_owned_addrs_def)
   done
 
-section \<open> Subset of accessible addresses \<close>
-
 \<comment> \<open>Address subset property: That only the paddrs of policy-accessible labels are ever accessed.\<close>
 definition ta_subset_accessible_addrs :: "'a PAS \<Rightarrow> det_state \<Rightarrow> bool" where
   "ta_subset_accessible_addrs aag s \<equiv>
@@ -130,10 +130,193 @@ lemma ta_subset_accessible_addrs_to_partitions_alternative:
   by (force intro:ta_subset_accessible_addrs_to_partitions
     owned_to_accessible_addrs_well_partitioned)
 
-\<comment> \<open>Proofs of TA subset invariance over seL4 kernel\<close>
+end
+
+section \<open> Subset property definitions that rely on the kernel heap status of objects \<close>
+
+context Arch begin
+
+\<comment> \<open> Adapted from Scott's definition of @{term\<open>touch_objects\<close>}.
+  I don't believe any existing definition gets the @{term\<open>obj_addrs\<close>}
+  conditionally on whether the object is on the @{term\<open>kheap\<close>} like this. -robs \<close>
+definition obj_kheap_addrs :: "'a state \<Rightarrow> obj_ref \<Rightarrow> machine_word set" where
+  "obj_kheap_addrs s p \<equiv> case kheap s p of
+     None \<Rightarrow> {} |
+     Some ko \<Rightarrow> obj_addrs ko p"
+
+\<comment> \<open>That no object is allocated on the @{term\<open>kheap\<close>} such that it straddles the addresses
+    assigned to two different labels according to @{term\<open>pasObjectAbs\<close>}}.\<close>
+definition no_label_straddling_objs :: "'a PAS \<Rightarrow> det_state \<Rightarrow> bool" where
+  "no_label_straddling_objs aag s \<equiv> \<forall>l p. pasObjectAbs aag p = l \<longrightarrow>
+     (case kheap s p of
+       Some ko \<Rightarrow> \<forall>va \<in> obj_addrs ko p. pasObjectAbs aag va = l |
+       None \<Rightarrow> True)"
+
+\<comment> \<open>New property discussed with Gerwin Klein (@lsf37) - haven't figured out its application yet.\<close>
+definition ta_obj_projections_subset_ta :: "det_state \<Rightarrow> bool" where
+  "ta_obj_projections_subset_ta  s \<equiv>
+     (\<Union> (obj_kheap_addrs s ` (touched_addresses (machine_state s)))) \<subseteq>
+     (touched_addresses (machine_state s)) "
+
+end
+
+context ArchL2Partitioned begin
+
+\<comment> \<open>That each domain's objects stay confined to that domain's partition.\<close>
+definition owned_objs_well_partitioned :: "'a PAS \<Rightarrow> det_state \<Rightarrow> bool" where
+  "owned_objs_well_partitioned aag s \<equiv> \<forall> d.
+     to_phys (\<Union> (obj_kheap_addrs s ` policy_owned_addrs aag d)) \<subseteq>
+     domain_L2_partition d"
+
+\<comment> \<open>That accessible objects will only lie inside accessible domains' partitions.\<close>
+definition accessible_objs_well_partitioned :: "'a PAS \<Rightarrow> det_state \<Rightarrow> bool" where
+  "accessible_objs_well_partitioned aag s \<equiv>
+     to_phys (\<Union> (obj_kheap_addrs s ` policy_accessible_addrs aag (cur_domain s))) \<subseteq>
+     policy_accessible_partitions aag (cur_domain s)"
+
+lemma accessible_objs_subset_accessible_addrs:
+  "no_label_straddling_objs aag s \<Longrightarrow>
+   to_phys (\<Union> (obj_kheap_addrs s ` policy_accessible_addrs aag (cur_domain s))) \<subseteq>
+   to_phys (policy_accessible_addrs aag (cur_domain s))"
+  unfolding no_label_straddling_objs_def
+  apply(clarsimp simp:obj_kheap_addrs_def image_def split:option.splits)
+  apply(rename_tac vas p va)
+  apply(rule_tac x=va in bexI)
+   apply force
+  apply(erule_tac x=p in allE)
+  apply(case_tac "kheap s p")
+   apply force
+  apply clarsimp
+  apply(erule_tac x=va in ballE)
+   apply(force simp:policy_accessible_addrs_def)
+  apply(force simp:policy_accessible_addrs_def)
+  done
+
+\<comment> \<open>That it's sufficient here to prove an invariant that's agnostic of colours, domains, etc.
+    rather than proving \<open>owned_objs_well_partitioned\<close> as an invariant directly.\<close>
+lemma owned_addrs_to_objs_well_partitioned:
+  "owned_addrs_well_partitioned aag \<Longrightarrow>
+   no_label_straddling_objs aag s \<Longrightarrow>
+   owned_objs_well_partitioned aag s"
+  unfolding owned_addrs_well_partitioned_def no_label_straddling_objs_def
+    owned_objs_well_partitioned_def
+  apply clarsimp
+  apply(rename_tac d va p)
+  apply(clarsimp simp:obj_kheap_addrs_def image_def split:option.splits)
+  apply(erule_tac x=d in allE)
+  apply(erule_tac x=p in allE)
+  apply clarsimp
+  apply(rename_tac d va p ko)
+  apply(erule_tac x=va in ballE)
+   apply(erule_tac c="addrFromKPPtr va" in subsetCE)
+    apply(clarsimp simp:policy_owned_addrs_def)
+    apply metis
+   apply force
+  apply force
+  done
+
+\<comment> \<open>If every domain's objects is confined to its partition, then all accessible objects, due to
+  belonging to accessible domains, are confined to the union of those domains' partitions. -robs\<close>
+lemma owned_to_accessible_objs_well_partitioned:
+  "\<lbrakk>all_labels_are_owned aag; owned_objs_well_partitioned aag s\<rbrakk> \<Longrightarrow>
+   accessible_objs_well_partitioned aag s"
+  unfolding accessible_objs_well_partitioned_def
+  apply clarsimp
+  apply(rename_tac va y)
+  \<comment> \<open>We consider each accessible object, call it \<open>y\<close>.\<close>
+  (* Things that matter for 'y' to be a valid object reference:
+     - It is allocated, i.e. kheap s y \<noteq> None.
+       This follows from the definition of obj_kheap_addrs. *)
+  \<comment> \<open>We know the L2 partitioning scheme assigns the physical address of \<open>y\<close> to some domain
+        \<open>paddr_L2_colour (addrFromKPPtr y)\<close>
+      But instead of that, we use the domain determined by the domain assignment
+      (via @{term\<open>pasDomainAbs\<close>}) of y's label (given by @{term\<open>pasObjectAbs\<close>}),
+      which @{term\<open>all_labels_are_owned\<close>} tells us exists.\<close>
+  apply(prop_tac "\<exists>yd. pasObjectAbs aag y \<in> pasDomainAbs aag yd")
+   apply(force simp:all_labels_are_owned_def)
+  apply(clarsimp simp:policy_accessible_partitions_def policy_accessible_domains_def)
+  apply(rule_tac x="domain_L2_partition yd" in exI)
+  apply(rule conjI)
+   apply(rule_tac x=yd in exI)
+   apply clarsimp
+   \<comment> \<open>Note: \<open>y \<in> policy_accessible_addrs aag (cur_domain s)\<close> is what tells
+       the intersection of the two sets is nonempty.\<close>
+   apply(erule_tac x=y in in_empty_interE)
+    apply(force simp:policy_owned_addrs_def)
+   apply force
+  apply(rename_tac va y yd)
+  \<comment> \<open>We now use @{term\<open>owned_objs_well_partitioned\<close>} to tell us \<open>y\<close> is in its domain's partition.\<close>
+  unfolding owned_objs_well_partitioned_def
+  apply(erule_tac x=yd in allE)
+  apply(subgoal_tac
+    "addrFromKPPtr va \<in> to_phys (\<Union> (obj_kheap_addrs s ` policy_owned_addrs aag yd))")
+   apply force
+  \<comment> \<open>Finally, \<open>va\<close> should be in the footprint of the @{term\<open>policy_owned_addrs\<close>} of \<open>yd\<close>
+      because that should include \<open>y\<close>.\<close>
+  apply(force simp:obj_kheap_addrs_def policy_owned_addrs_def)
+  done
+
+\<comment> \<open>Object subset property: That only the paddrs of policy-accessible objects are ever accessed.\<close>
+definition ta_subset_accessible_objects :: "'a PAS \<Rightarrow> det_state \<Rightarrow> bool" where
+  "ta_subset_accessible_objects aag s \<equiv>
+     phys_touched s \<subseteq>
+     to_phys (\<Union> (obj_kheap_addrs s ` policy_accessible_addrs aag (cur_domain s)))"
+
+(* If it is easier to prove `ta_subset_accessible_objects` than
+   `ta_subset_accessible_addrs` as an invariant,
+   then we need `no_label_straddling_objs` as an invariant too. *)
+lemma ta_subset_accessible_objs_to_addrs:
+  "ta_subset_accessible_objects aag s \<Longrightarrow>
+   no_label_straddling_objs aag s \<Longrightarrow>
+   ta_subset_accessible_addrs aag s"
+  unfolding ta_subset_accessible_addrs_def ta_subset_accessible_objects_def
+  using accessible_objs_subset_accessible_addrs
+  by blast
+
+(* This is one potential way to get from `ta_subset_accessible_objects` to
+   `ta_subset_accessible_partitions`.
+   But we wouldn't want to prove `accessible_objs_well_partitioned` invariant directly
+   because it depends on the state of the `kheap`. *)
+lemma ta_subset_accessible_objs_to_partitions_HARD:
+  "ta_subset_accessible_objects aag s \<Longrightarrow>
+   accessible_objs_well_partitioned aag s \<Longrightarrow>
+   ta_subset_accessible_partitions aag s"
+  unfolding ta_subset_accessible_partitions_def ta_subset_accessible_objects_def
+    accessible_objs_well_partitioned_def
+  by blast
+
+(* We can avoid proving `accessible_objs_well_partitioned` (which depends on the kheap)
+   if it's straightforward enough to prove `accessible_addrs_well_partitioned`,
+   but in exchange we need to prove `no_label_straddling_objs`. *)
+theorem ta_subset_accessible_objs_to_partitions:
+  "ta_subset_accessible_objects aag s \<Longrightarrow>
+   no_label_straddling_objs aag s \<Longrightarrow>
+   accessible_addrs_well_partitioned aag \<Longrightarrow>
+   ta_subset_accessible_partitions aag s"
+  apply(drule ta_subset_accessible_objs_to_addrs)
+   apply force
+  apply(drule ta_subset_accessible_addrs_to_partitions)
+   apply force
+  apply force
+  done
+
+(* Finally, if it's easier to prove `owned_addrs_well_partitioned` than
+   `accessible_addrs_well_partitioned` then we'll additionally need `all_labels_are_owned`.
+   Though, again, the difference in difficulty between the two is questionable because
+   neither of them depend on the state anyway. *)
+lemma ta_subset_accessible_objs_to_partitions_alternative:
+  "ta_subset_accessible_objects aag s \<Longrightarrow>
+   no_label_straddling_objs aag s \<Longrightarrow>
+   all_labels_are_owned aag \<Longrightarrow>
+   owned_addrs_well_partitioned aag \<Longrightarrow>
+   ta_subset_accessible_partitions aag s"
+  by (force intro:ta_subset_accessible_objs_to_partitions_HARD
+    owned_addrs_to_objs_well_partitioned owned_to_accessible_objs_well_partitioned)
+
+section \<open>Proofs of TA subset invariance over seL4 kernel\<close>
 
 abbreviation ta_subset_inv :: "'a PAS \<Rightarrow> det_state \<Rightarrow> bool" where
-  "ta_subset_inv \<equiv> ta_subset_accessible_addrs"
+  "ta_subset_inv \<equiv> ta_subset_accessible_addrs" \<comment> \<open>Right now we're trying the kheap-agnostic one.\<close>
 
 (* For check_active_irq_if *)
 
@@ -151,6 +334,7 @@ lemma syscall_ta_subset_inv:
   "syscall m_fault h_fault m_error h_error m_finalise \<lbrace>ta_subset_inv aag\<rbrace>"
   sorry
 
+(* Scott (@scottbuckley) recommends trying to prove this one -robs. *)
 lemma resolve_address_bits'_ta_subset_inv:
   "resolve_address_bits' z capcref \<lbrace>ta_subset_inv aag\<rbrace>"
   sorry
